src/TaggedComp.v
@@ -1,4 +1,5 @@
 Require Import Common.
+Require Import Psatz.
 
 Require Import Monads.
 Require Import StuartTact.
@@ -10,22 +11,23 @@ Require Utopia String.
 Require Lifted.
 Require Tagged.
 
-Module L := Lifted.
-Module T := Tagged.
+Module A := Lifted.
+Module B := Tagged.
 
 
 Section compile.
 Open Scope option_monad.
 
-Definition mk_rec_info ctor :=
-    let fix go acc n :=
-        match n with
-        | 0 => acc
-        | S n => go (Utopia.ctor_arg_is_recursive ctor n :: acc) n
-        end in
-    go [] (Utopia.constructor_arg_n ctor).
+Fixpoint mk_rec_info' ctor acc n :=
+    match n with
+    | 0 => acc
+    | S n => mk_rec_info' ctor (Utopia.ctor_arg_is_recursive ctor n :: acc) n
+    end.
 
-Fixpoint mk_tagged_cases' ty idx cases : option (list (T.expr * T.rec_info)) :=
+Definition mk_rec_info ctor :=
+    mk_rec_info' ctor [] (Utopia.constructor_arg_n ctor).
+
+Fixpoint mk_tagged_cases' ty idx cases : option (list (B.expr * B.rec_info)) :=
     match cases with
     | [] => Some []
     | case :: cases =>
@@ -37,7 +39,7 @@ Fixpoint mk_tagged_cases' ty idx cases : option (list (T.expr * T.rec_info)) :=
 Definition mk_tagged_cases ty cases :=
     mk_tagged_cases' ty 0 cases.
 
-Definition compile (e : L.expr) : option T.expr :=
+Definition compile (e : A.expr) : option B.expr :=
     let fix go e :=
         let fix go_list es :=
             match es with
@@ -45,25 +47,25 @@ Definition compile (e : L.expr) : option T.expr :=
             | e :: es => cons <$> go e <*> go_list es
             end in
         match e with
-        | L.Arg => Some (T.Arg)
-        | L.UpVar n => Some (T.UpVar n)
-        | L.Call f a => T.Call <$> go f <*> go a
-        | L.Constr c args => T.Constr (Utopia.constructor_index c) <$> go_list args
-        | L.Elim ty cases target =>
+        | A.Arg => Some (B.Arg)
+        | A.UpVar n => Some (B.UpVar n)
+        | A.Call f a => B.Call <$> go f <*> go a
+        | A.Constr c args => B.Constr (Utopia.constructor_index c) <$> go_list args
+        | A.Elim ty cases target =>
                 go_list cases >>= fun cases =>
-                T.Elim <$> mk_tagged_cases ty cases <*> go target
-        | L.Close f free => T.Close f <$> go_list free
+                B.Elim <$> mk_tagged_cases ty cases <*> go target
+        | A.Close f free => B.Close f <$> go_list free
         end in go e.
 
 (* Nested fixpoint alias for `compile`, but also used as a top-level function *)
 Definition compile_list :=
-    let fix go_list (es : list L.expr) : option (list T.expr) :=
+    let fix go_list (es : list A.expr) : option (list B.expr) :=
         match es with
         | [] => Some []
         | e :: es => cons <$> compile e <*> go_list es
         end in go_list.
 
-Definition compile_cu (cu : list L.expr * list metadata) : option (list T.expr * list metadata) :=
+Definition compile_cu (cu : list A.expr * list metadata) : option (list B.expr * list metadata) :=
     let '(exprs, metas) := cu in
     compile_list exprs >>= fun exprs' =>
     Some (exprs', metas).
@@ -74,51 +76,418 @@ Ltac refold_compile := fold compile_list in *.
 Ltac simpl_compile := simpl in *; refold_compile.
 
 
-(* spec *)
 
-Inductive R (LE : L.env) (TE : T.env) : L.expr -> T.expr -> Prop :=
-| RConstr : forall c largs targs,
-        Forall2 (R LE TE) largs targs ->
-        R LE TE
-            (L.Constr c largs)
-            (T.Constr (Utopia.constructor_index c) targs)
-| RClose : forall fn lf tf lfree tfree,
-        nth_error LE fn = Some lf ->
-        nth_error TE fn = Some tf ->
-        compile lf = Some tf ->
-        Forall2 (R LE TE) lfree tfree ->
-        R LE TE
-            (L.Close fn lfree)
-            (T.Close fn tfree)
+Lemma mk_rec_info'_length : forall ctor acc n,
+    length (mk_rec_info' ctor acc n) = length acc + n.
+first_induction n; intros; simpl.
+- lia.
+- rewrite IHn. simpl. lia.
+Qed.
+
+Lemma mk_rec_info_length : forall ctor,
+    length (mk_rec_info ctor) = Utopia.constructor_arg_n ctor.
+intros. unfold mk_rec_info. rewrite mk_rec_info'_length.
+simpl. lia.
+Qed.
+
+Lemma mk_rec_info'_spec : forall ctor acc n rec,
+    (forall i b,
+        nth_error acc i = Some b ->
+        b = Utopia.ctor_arg_is_recursive ctor (n + i)) ->
+    mk_rec_info' ctor acc n = rec ->
+    (forall i b,
+        nth_error rec i = Some b ->
+        b = Utopia.ctor_arg_is_recursive ctor i).
+first_induction n; intros0 Hi Hrec; simpl in *.
+- intros. eapply Hi. congruence.
+- eapply IHn; try eassumption.
+  intros. destruct i.
+  + simpl in *. replace (n + 0) with n by lia. congruence.
+  + replace (n + S i) with (S (n + i)) by lia. eapply Hi. eauto.
+Qed.
+
+Lemma mk_rec_info_spec : forall ctor rec,
+    mk_rec_info ctor = rec ->
+    (forall i b,
+        nth_error rec i = Some b ->
+        b = Utopia.ctor_arg_is_recursive ctor i).
+intros0 Hrec.
+eapply mk_rec_info'_spec; try eassumption.
+intros. destruct i; discriminate.
+Qed.
+
+Lemma mk_tagged_cases'_length : forall ty idx cases cases',
+    mk_tagged_cases' ty idx cases = Some cases' ->
+    length cases = length cases'.
+first_induction cases; destruct cases'; intros;
+simpl in *; break_bind_option; try discriminate.
+- reflexivity.
+- on (Some _ = Some _), invc.
+  f_equal. eapply IHcases. eauto.
+Qed.
+
+Lemma mk_tagged_cases_length : forall ty cases cases',
+    mk_tagged_cases ty cases = Some cases' ->
+    length cases = length cases'.
+intros. eapply mk_tagged_cases'_length; eauto.
+Qed.
+
+Lemma compile_list_length : forall aes bes,
+    compile_list aes = Some bes ->
+    length aes = length bes.
+induction aes; destruct bes; intros;
+simpl in *; break_bind_option; inject_some; try discriminate.
+- reflexivity.
+- on (_ :: _ = _ :: _), invc.
+  f_equal. eauto.
+Qed.
+
+
+
+Inductive I_expr : A.expr -> B.expr -> Prop :=
+| IArg : I_expr A.Arg B.Arg
+| IUpVar : forall n,
+        I_expr (A.UpVar n) (B.UpVar n)
+| ICall : forall af aa bf ba,
+        I_expr af bf ->
+        I_expr aa ba ->
+        I_expr (A.Call af aa) (B.Call bf ba)
+| IConstr : forall ctor aargs tag bargs,
+        Utopia.constructor_index ctor = tag ->
+        Forall2 I_expr aargs bargs ->
+        I_expr (A.Constr ctor aargs) (B.Constr tag bargs)
+| IElim : forall aty acases atarget bcases btarget,
+        length acases = length bcases ->
+        (forall i acase bcase brec ctor,
+            nth_error acases i = Some acase ->
+            nth_error bcases i = Some (bcase, brec) ->
+            Utopia.type_constr aty i = Some ctor ->
+            I_expr acase bcase /\
+            brec = mk_rec_info ctor) ->
+        I_expr atarget btarget ->
+        I_expr (A.Elim aty acases atarget)
+               (B.Elim bcases btarget)
+| IClose : forall tag afree bfree,
+        Forall2 I_expr afree bfree ->
+        I_expr (A.Close tag afree) (B.Close tag bfree)
 .
 
+Inductive I : A.state -> B.state -> Prop :=
+| IRun : forall ae al ak be bl bk,
+        I_expr ae be ->
+        Forall A.value al ->
+        Forall B.value bl ->
+        Forall2 I_expr al bl ->
+        (forall av bv,
+            A.value av ->
+            B.value bv ->
+            I_expr av bv ->
+            I (ak av) (bk bv)) ->
+        I (A.Run ae al ak) (B.Run be bl bk)
 
-(* induction hypothesis *)
+| IStop : forall ae be,
+        I_expr ae be ->
+        I (A.Stop ae) (B.Stop be).
 
-Definition I l t := compile l = Some t.
-Hint Unfold I.
 
+
+Lemma I_expr_value : forall a b,
+    I_expr a b ->
+    A.value a ->
+    B.value b.
+induction a using A.expr_ind'; intros0 II Aval; invc Aval; invc II.
+- constructor. list_magic_on (args, (bargs, tt)).
+- constructor. list_magic_on (free, (bfree, tt)).
+Qed.
+Hint Resolve I_expr_value.
+
+Lemma I_expr_value' : forall b a,
+    I_expr a b ->
+    B.value b ->
+    A.value a.
+induction b using B.expr_ind''; intros0 II Bval; invc Bval; invc II.
+- constructor. list_magic_on (args, (aargs, tt)).
+- constructor. list_magic_on (free, (afree, tt)).
+Qed.
+
+Lemma I_expr_not_value : forall a b,
+    I_expr a b ->
+    ~A.value a ->
+    ~B.value b.
+intros. intro. fwd eapply I_expr_value'; eauto.
+Qed.
+Hint Resolve I_expr_not_value.
+
+Lemma I_expr_not_value' : forall a b,
+    I_expr a b ->
+    ~B.value b ->
+    ~A.value a.
+intros. intro. fwd eapply I_expr_value; eauto.
+Qed.
+
+Lemma Forall_I_expr_value : forall aes bes,
+    Forall2 I_expr aes bes ->
+    Forall A.value aes ->
+    Forall B.value bes.
+intros. list_magic_on (aes, (bes, tt)).
+Qed.
+Hint Resolve Forall_I_expr_value.
+
+
+
+(* compile_I_expr *)
+
+Lemma mk_tagged_cases'_I_expr : forall ty acases bcases0 bcases idx,
+    Forall2 I_expr acases bcases0 ->
+    mk_tagged_cases' ty idx bcases0 = Some bcases ->
+    forall i acase bcase brec ctor,
+    nth_error acases i = Some acase ->
+    nth_error bcases i = Some (bcase, brec) ->
+    Utopia.type_constr ty (idx + i) = Some ctor ->
+    I_expr acase bcase /\ brec = mk_rec_info ctor.
+first_induction acases; intros0 Hcomp Htag.
+  { intros. destruct i; discriminate. }
+on (Forall2 _ (_ :: _) _), invc.
+simpl in *. break_bind_option. inject_some.
+specialize (IHacases ?? ?? ?? ?? *** **).
+
+intros. destruct i. simpl in *.
+  { replace (idx + 0) with idx in * by lia.  split; congruence. }
+eapply IHacases; eauto.
+- replace (S idx + i) with (idx + S i) by lia.
+  assumption.
+Qed.
+
+Lemma mk_tagged_cases_I_expr : forall ty acases bcases0 bcases,
+    Forall2 I_expr acases bcases0 ->
+    mk_tagged_cases ty bcases0 = Some bcases ->
+    forall i acase bcase brec ctor,
+    nth_error acases i = Some acase ->
+    nth_error bcases i = Some (bcase, brec) ->
+    Utopia.type_constr ty i = Some ctor ->
+    I_expr acase bcase /\ brec = mk_rec_info ctor.
+intros. eapply mk_tagged_cases'_I_expr; eauto.
+Qed.
+
+Theorem compile_I_expr : forall ae be,
+    compile ae = Some be ->
+    I_expr ae be.
+induction ae using A.expr_rect_mut with
+    (Pl := fun aes => forall bes,
+        compile_list aes = Some bes ->
+        Forall2 I_expr aes bes);
+intros0 Hcomp;
+simpl in Hcomp; refold_compile; try rewrite <- Hcomp in *;
+break_bind_option; inject_some; try solve [eauto | econstructor; eauto].
+
+- (* elim case *)
+  econstructor; eauto.
+  + erewrite compile_list_length by eauto.
+    eauto using mk_tagged_cases_length.
+  + eapply mk_tagged_cases_I_expr; eauto.
+Qed.
+
+
+
+(* I_sim *)
+
+Ltac i_ctor := intros; constructor; eauto.
+Ltac i_lem H := intros; eapply H; eauto.
+
+Lemma skipn_all : forall A n (xs : list A),
+    n >= length xs ->
+    skipn n xs = [].
+first_induction xs; intros0 Hlen.
+- destruct n; reflexivity.
+- destruct n; simpl in *.  { lia. }
+  eapply IHxs. lia.
+Qed.
+
+Lemma skipn_all' : forall A n (xs : list A),
+    skipn n xs = [] ->
+    n >= length xs.
+first_induction xs; intros0 Hlen.
+- destruct n; simpl in *; try discriminate; lia.
+- destruct n; simpl in *; try discriminate.
+  specialize (IHxs ?? **).
+  lia.
+Qed.
+
+Lemma unroll'_sim :
+    forall acase actor aargs amk_rec aidx ae',
+    forall bcase bargs brec bmk_rec,
+    A.unroll_elim' acase actor aargs amk_rec aidx = ae' ->
+    I_expr acase bcase ->
+    Forall2 I_expr aargs bargs ->
+    skipn aidx (mk_rec_info actor) = brec ->
+    (forall av bv,
+        I_expr av bv ->
+        I_expr (amk_rec av) (bmk_rec bv)) ->
+    aidx + length aargs = Utopia.constructor_arg_n actor ->
+    exists be',
+        B.unroll_elim bcase bargs brec bmk_rec = Some be' /\
+        I_expr ae' be'.
+first_induction aargs; intros0 Aunroll IIcase IIargs IIrec IImk_rec IIidx;
+simpl in *.
+
+- on (Forall2 _ [] _), invc.
+  rewrite skipn_all; [ | rewrite mk_rec_info_length; lia ].
+  simpl. eauto.
+
+- on (Forall2 _ (_ :: _) _), invc.
+  fwd eapply mk_rec_info_length with (ctor := actor).
+
+  destruct (skipn _ _) eqn:Hskip.
+    { eapply skipn_all' in Hskip. lia. }
+
+  rewrite skipn_slice in Hskip.
+  rewrite slice_split with (k := S aidx) in Hskip by lia.
+  assert (nth_error (mk_rec_info actor) aidx <> None).
+    { rewrite nth_error_Some. lia. }
+  destruct (nth_error (mk_rec_info actor) aidx) eqn:?; try congruence.
+  erewrite nth_error_slice in Hskip by eassumption. simpl in Hskip. invc Hskip.
+
+  fwd eapply mk_rec_info_spec; eauto. subst b.
+
+  simpl. eapply IHaargs; eauto using skipn_slice; try lia.
+  destruct (Utopia.ctor_arg_is_recursive); repeat i_ctor.
+Qed.
+
+Lemma unroll_sim :
+    forall acase actor aargs amk_rec ae',
+    forall bcase bargs brec bmk_rec,
+    A.unroll_elim acase actor aargs amk_rec = ae' ->
+    I_expr acase bcase ->
+    Forall2 I_expr aargs bargs ->
+    mk_rec_info actor = brec ->
+    length aargs = Utopia.constructor_arg_n actor ->
+    (forall av bv,
+        I_expr av bv ->
+        I_expr (amk_rec av) (bmk_rec bv)) ->
+    exists be',
+        B.unroll_elim bcase bargs brec bmk_rec = Some be' /\
+        I_expr ae' be'.
+intros. eapply unroll'_sim; eauto.
+Qed.
+
+Theorem I_sim : forall AE BE a a' b,
+    Forall2 I_expr AE BE ->
+    I a b ->
+    A.sstep AE a a' ->
+    exists b',
+        B.sstep BE b b' /\
+        I a' b'.
+
+destruct a as [ae al ak | ae];
+intros0 Henv II Astep; [ | solve [invc Astep] ].
+
+inv Astep; invc II; try on (I_expr _ _), invc.
+
+- fwd eapply Forall2_nth_error_ex with (xs := al) (ys := bl); eauto.
+    break_exists. break_and.
+  assert (A.value v).  { eapply Forall_nth_error; eauto. }
+
+  eexists. split. eapply B.SArg; eauto.
+  on _, eapply_; eauto.
+
+- fwd eapply Forall2_nth_error_ex with (xs := al) (ys := bl); eauto.
+    break_exists. break_and.
+  assert (A.value v).  { eapply Forall_nth_error; eauto. }
+
+  eexists. split. eapply B.SUpVar; eauto.
+  on _, eapply_; eauto.
+
+- on _, invc_using Forall2_3part_inv.
+
+  eexists. split. eapply B.SCloseStep; eauto.
+  i_ctor. i_ctor. i_ctor. eauto using Forall2_app.
+
+- eexists. split. eapply B.SCloseDone; eauto.
+  on _, eapply_; eauto.
+  all: constructor; eauto.
+
+- on _, invc_using Forall2_3part_inv.
+
+  eexists. split. eapply B.SConstrStep; eauto.
+  i_ctor. i_ctor. i_ctor. eauto using Forall2_app.
+
+- eexists. split. eapply B.SConstrDone; eauto.
+  on _, eapply_; eauto.
+  all: constructor; eauto.
+
+- eexists. split. eapply B.SCallL; eauto.
+  i_ctor. i_ctor. i_ctor.
+
+- eexists. split. eapply B.SCallR; eauto.
+  i_ctor. i_ctor. i_ctor.
+
+- fwd eapply Forall2_nth_error_ex with (xs := AE) (ys := BE) as HH; eauto.
+    destruct HH as (bbody & ? & ?).
+  on (I_expr (A.Close _ _) _), invc.
+
+  eexists. split. eapply B.SMakeCall; eauto.
+  i_ctor.
+
+- eexists. split. eapply B.SElimStep; eauto.
+  i_ctor. i_ctor. i_ctor.
+
+- fwd eapply length_nth_error_Some as HH; try eassumption.
+    destruct HH as ([bcase brec] & ?).
+  on (I_expr _ btarget), invc.
+  remember (A.unroll_elim _ _ _ _) as e'. symmetry in Heqe'.
+
+  pose proof H13 as Hnth.
+  specialize (Hnth ?? ?? ?? ?? c ** ** ltac:(eauto using Utopia.ctor_for_type_constr_index)).
+  break_and.
+  subst brec.
+
+  fwd eapply unroll_sim; eauto. { i_ctor. }
+    break_exists. break_and.
+
+  eexists. split. eapply B.SEliminate; eauto.
+  i_ctor.
+Qed.
+
+
+
+(* spec *)
+
+Inductive R (AE : A.env) (BE : B.env) : A.expr -> B.expr -> Prop :=
+| RConstr : forall c aargs bargs,
+        Forall2 (R AE BE) aargs bargs ->
+        R AE BE
+            (A.Constr c aargs)
+            (B.Constr (Utopia.constructor_index c) bargs)
+| RClose : forall fn af bf afree bfree,
+        nth_error AE fn = Some af ->
+        nth_error BE fn = Some bf ->
+        compile af = Some bf ->
+        Forall2 (R AE BE) afree bfree ->
+        R AE BE
+            (A.Close fn afree)
+            (B.Close fn bfree)
+.
 
 Section Preservation.
 
-  (* Variable prog : list L.expr * list metadata. *)
-  (* Variable tprog : list T.expr * list metadata. *)
+  (* Variable prog : list A.expr * list metadata. *)
+  (* Variable tprog : list B.expr * list metadata. *)
 
   (* Hypothesis TRANSF : compile_cu prog = Some tprog. *)
 
-  Inductive match_states (LE : L.env) (TE : T.env) : L.expr -> T.expr -> Prop :=
+  Inductive match_states (AE : A.env) (BE : B.env) : A.expr -> B.expr -> Prop :=
   | match_st :
-      forall l t,
-        R LE TE l t ->
-        match_states LE TE l t.
+      forall a b,
+        R AE BE a b ->
+        match_states AE BE a b.
 
   Lemma step_sim :
-    forall LE TE l t,
-      match_states LE TE l t ->
-      forall l',
-        L.step LE l l' ->
-        exists t',
-          splus (T.step TE) t t'.
+    forall AE BE a b,
+      match_states AE BE a b ->
+      forall a',
+        A.step AE a a' ->
+        exists b',
+          splus (B.step BE) b b'.
   Proof.
   Admitted.
 
